theories/Block/vst/verif/vsu.v
@@ -1,0 +1,28 @@
+From VST Require Import floyd.proofauto.
+From VST Require Import floyd.VSU.
+
+From CertiCoq Require Import Block.vst.clightgen.block.
+From CertiCoq Require Import Block.vst.spec.spec.
+From CertiCoq Require Import Block.vst.verif.certicoq_block__copy.
+From CertiCoq Require Import Block.vst.verif.certicoq_block__field_count_get.
+From CertiCoq Require Import Block.vst.verif.certicoq_block__field_count_set.
+From CertiCoq Require Import Block.vst.verif.certicoq_block__field_get_ptr.
+From CertiCoq Require Import Block.vst.verif.certicoq_block__field_iter.
+From CertiCoq Require Import Block.vst.verif.certicoq_block__field_ptr_iter.
+From CertiCoq Require Import Block.vst.verif.certicoq_block__header_get_ptr.
+From CertiCoq Require Import Block.vst.verif.certicoq_block__init.
+From CertiCoq Require Import Block.vst.verif.certicoq_block__odata_get.
+From CertiCoq Require Import Block.vst.verif.certicoq_block__odata_set.
+From CertiCoq Require Import Block.vst.verif.certicoq_block__of_header.
+From CertiCoq Require Import Block.vst.verif.certicoq_block__size_get.
+From CertiCoq Require Import Block.vst.verif.certicoq_block__tag_get.
+From CertiCoq Require Import Block.vst.verif.certicoq_block__tag_is_noscan.
+From CertiCoq Require Import Block.vst.verif.certicoq_block__tag_noscan_limit.
+From CertiCoq Require Import Block.vst.verif.certicoq_block__tag_set.
+
+#[local] Existing Instance NullExtension.Espec.
+
+Lemma certicoq_block__vsu: VSU certicoq_block__specs.externs certicoq_block__specs.imports ltac:(QPprog prog) certicoq_block__specs.exports emp.
+Proof.
+  mkVSU prog certicoq_block__specs.all.
+Admitted.
